Loop body seems to be inductive

src/crypto/aes/x64/Low.GCMencrypt.fst
@@ -305,7 +305,7 @@ assume val gcm_load_xor_store_buffer
      let cipher = buffer_to_seq_quad32 cipher_b h' in
      let key = Ghost.reveal key in
      let iv = Ghost.reveal iv in
-     gctr_partial AES_128 (offset + 1) plain cipher key (inc32 iv (offset + 1))
+     gctr_partial AES_128 (offset + 1) plain cipher key iv
     ) /\
   True) 
 
@@ -321,6 +321,13 @@ assume val inc32_buffer (iv_b:B.buffer U8.t) : Stack unit
      new_iv == inc32 old_iv 1))
 
 (*** Actual Low* code ***)
+
+let inc32_twice (q:quad32) (i:int) :
+  Lemma (inc32 (inc32 q i) 1 == inc32 q (i + 1))
+  =
+  ()
+
+#reset-options "--z3rlimit 20"
 let gcm128_one_pass_blocks 
              (plain_b:B.buffer U8.t) (num_blocks:U32.t)  
              (iv_b:B.buffer U8.t) 
@@ -337,6 +344,9 @@ let gcm128_one_pass_blocks
     M.loc_disjoint (M.loc_buffer plain_b) mods /\
     M.loc_disjoint (M.loc_buffer keys_b)  mods /\
     M.loc_disjoint (M.loc_buffer h_b)  mods /\
+    M.(loc_disjoint (loc_buffer cipher_b) (loc_buffer   iv_b)) /\
+    M.(loc_disjoint (loc_buffer cipher_b) (loc_buffer hash_b)) /\ 
+    M.(loc_disjoint (loc_buffer iv_b)     (loc_buffer hash_b)) /\
     B.length plain_b  >= U32.v num_blocks * 16 /\
     B.length cipher_b == B.length plain_b /\
     B.length iv_b == 16 /\
@@ -370,8 +380,8 @@ let gcm128_one_pass_blocks
          )
        )
       )
-    ) /\
-  True) 
+    )
+  ) 
   =
   push_frame();
 //  let ctr_b = B.alloca 0uy 16ul in
@@ -407,19 +417,49 @@ let gcm128_one_pass_blocks
   in
   let body (i:U32.t{ U32.v 0ul <= U32.v i /\ U32.v i < U32.v num_blocks }) : Stack unit
     (requires (fun h -> inv h (U32.v i)))
-    (ensures (fun h () h' -> inv h (U32.v i) /\ inv h (U32.v i + 1)))
+    (ensures (fun h () h' -> inv h (U32.v i) /\ inv h' (U32.v i + 1)))
     =
-    aes128_encrypt_block_buffer iv_b enc_ctr_b key keys_b;
     let h1 = ST.get() in
+    // Compute the encryption of the counter value
+    aes128_encrypt_block_buffer iv_b enc_ctr_b key keys_b;
+    let h2 = ST.get() in
+    
+    let j = U32.v i in
+assert (let old_iv = buffer_to_quad32 iv_b h0 in
+    buffer_to_quad32 enc_ctr_b h2 == aes_encrypt_LE AES_128 (Ghost.reveal key) (inc32 old_iv j));
+    
+    // Xor the encrypted counter to the plaintext, to make progress on the gctr computation
     let iv = Ghost.elift2 buffer_to_quad32 (Ghost.hide iv_b) (Ghost.hide h0) in
     gcm_load_xor_store_buffer plain_b enc_ctr_b cipher_b i (Ghost.hide num_blocks) key iv;
+    let h3 = ST.get() in
+    assert (
+    let old_iv = buffer_to_quad32 iv_b h0 in
+            let plain  = buffer_to_seq_quad32  plain_b h3 in
+            let cipher = buffer_to_seq_quad32 cipher_b h3 in
+    gctr_partial AES_128 (j + 1) plain cipher (Ghost.reveal key) old_iv);
+    
+(*
+    assert (let old_iv = buffer_to_quad32 iv_b h0 in
+            let plain  = buffer_to_seq_quad32  plain_b h3 in
+            let cipher = buffer_to_seq_quad32 cipher_b h3 in
+      index cipher j == quad32_xor (index plain j) (aes_encrypt_LE AES_128 (Ghost.reveal key) (inc32 old_iv j)));
+      *)
 
     // Update our hash
-    //ghash_incremental_bytes_buffer h_b hash_b cipher_b
+    let i32:nat32 = UInt32.v i in
+    let i64:UInt64.t = UInt64.uint_to_t i32 in
+    ghash_incremental_one_block_buffer h_b hash_b cipher_b i64;
+    let h4 = ST.get() in
+    assert (buffer_to_quad32 iv_b h3 == buffer_to_quad32 iv_b h4);
 
     // Increment the ctr
     inc32_buffer iv_b;
-    admit();
+    let h5 = ST.get() in
+
+    // Help with the calculation showing we incremented iv_b correctly
+    //inc32_twice (buffer_to_quad32 iv_b h0) (U32.v i);
+    //assert (buffer_to_quad32 iv_b h5 == inc32 (buffer_to_quad32 iv_b h0) ((U32.v i) + 1));
+    let j = i32 in
     ()
   in
   //C.Loops.for 0ul num_blocks inv body;
